common/Common.ProtocolEndpoint.fst
@@ -1,0 +1,591 @@
+module Common.ProtocolEndpoint
+
+#lang-pulse
+
+open Pulse.Lib.Pervasives
+
+module CPI = Common.ProtocolImplementation
+module Seq = FStar.Seq
+module SZ = FStar.SizeT
+module TCP = Common.TCP
+module U8 = FStar.UInt8
+
+type endpoint_action
+  (network_frame:Type0)
+  (local_event:Type0)
+  (local_frame:Type0)
+  =
+  | EndpointNeedInput:
+      frame:network_frame ->
+        endpoint_action network_frame local_event local_frame
+  | EndpointLocal:
+      ev:local_event ->
+      frame:local_frame ->
+        endpoint_action network_frame local_event local_frame
+  | EndpointDone:
+        endpoint_action network_frame local_event local_frame
+  | EndpointFailed:
+        endpoint_action network_frame local_event local_frame
+
+[@@pulse_unfold]
+let network_buffers
+  (input:array U8.t)
+  (input_len:SZ.t)
+  (out:array U8.t)
+  (out_len:SZ.t)
+  (input_contents:TCP.bytes)
+  (old_out:TCP.bytes)
+  : slprop =
+  pts_to input input_contents **
+  pts_to out old_out **
+  pure (
+    Seq.length input_contents == SZ.v input_len /\
+    Seq.length old_out == SZ.v out_len)
+
+[@@pulse_unfold]
+let local_output_buffer
+  (out:array U8.t)
+  (out_len:SZ.t)
+  (old_out:TCP.bytes)
+  : slprop =
+  pts_to out old_out **
+  pure (Seq.length old_out == SZ.v out_len)
+
+noextract
+class protocol_endpoint
+  (impl:Type0)
+  (state:Type0)
+  (wire_message:Type0)
+  (local_event:Type0)
+  (local_output:Type0)
+  (protocol:CPI.protocol_implementation
+    impl
+    state
+    wire_message
+    local_event
+    local_output)
+  =
+{
+  pe_channel:
+    Type0;
+
+  pe_config:
+    Type0;
+
+  pe_frame:
+    Type0;
+
+  pe_frame_ready:
+    impl ->
+    pe_config ->
+    pe_frame ->
+    state ->
+    slprop;
+
+  pe_io_ready:
+    impl ->
+    pe_channel ->
+    pe_frame ->
+    TCP.bytes ->
+    TCP.bytes ->
+    state ->
+    slprop;
+
+  pe_action_frame:
+    impl ->
+    pe_config ->
+    pe_frame ->
+    state ->
+    endpoint_action
+      protocol.CPI.pi_network_frame
+      local_event
+      protocol.CPI.pi_local_frame ->
+    slprop;
+
+  pe_network_continuation:
+    impl ->
+    pe_config ->
+    pe_frame ->
+    state ->
+    protocol.CPI.pi_network_frame ->
+    slprop;
+
+  pe_local_continuation:
+    impl ->
+    pe_config ->
+    pe_frame ->
+    state ->
+    local_event ->
+    protocol.CPI.pi_local_frame ->
+    slprop;
+
+  pe_next_action:
+    i:impl ->
+    cfg:pe_config ->
+    frame:pe_frame ->
+    received:Ghost.erased TCP.bytes ->
+    sent:Ghost.erased TCP.bytes ->
+    st:Ghost.erased state ->
+      stt (endpoint_action
+        protocol.CPI.pi_network_frame
+        local_event
+        protocol.CPI.pi_local_frame)
+        (protocol.CPI.pi_invariant
+           i
+           (Ghost.reveal received)
+           (Ghost.reveal sent)
+           (Ghost.reveal st) **
+         pe_frame_ready
+           i
+           cfg
+           frame
+           (Ghost.reveal st))
+        (fun action ->
+          protocol.CPI.pi_invariant
+            i
+            (Ghost.reveal received)
+            (Ghost.reveal sent)
+            (Ghost.reveal st) **
+          pe_action_frame
+            i
+            cfg
+            frame
+            (Ghost.reveal st)
+            action);
+
+  pe_cancel_action:
+    i:impl ->
+    cfg:pe_config ->
+    frame:pe_frame ->
+    st:Ghost.erased state ->
+    action:endpoint_action
+      protocol.CPI.pi_network_frame
+      local_event
+      protocol.CPI.pi_local_frame ->
+      stt unit
+        (pe_action_frame
+          i
+          cfg
+          frame
+          (Ghost.reveal st)
+          action)
+        (fun _ ->
+          pe_frame_ready
+            i
+            cfg
+            frame
+            (Ghost.reveal st));
+
+  pe_prepare_network_action:
+    i:impl ->
+    cfg:pe_config ->
+    frame:pe_frame ->
+    network_frame:protocol.CPI.pi_network_frame ->
+    input:array U8.t ->
+    input_len:SZ.t ->
+    out:array U8.t ->
+    out_len:SZ.t ->
+    st:Ghost.erased state ->
+    input_contents:Ghost.erased TCP.bytes ->
+    old_out:Ghost.erased TCP.bytes ->
+      stt unit
+        (pe_action_frame
+          i
+          cfg
+          frame
+          (Ghost.reveal st)
+          (EndpointNeedInput network_frame) **
+         network_buffers
+          input
+          input_len
+          out
+          out_len
+          (Ghost.reveal input_contents)
+          (Ghost.reveal old_out))
+        (fun _ ->
+          protocol.CPI.pi_network_frame_pre
+            network_frame
+            input
+            input_len
+            out
+            out_len
+            (Ghost.reveal input_contents)
+            (Ghost.reveal old_out) **
+          pe_network_continuation
+            i
+            cfg
+            frame
+            (Ghost.reveal st)
+            network_frame **
+          network_buffers
+            input
+            input_len
+            out
+            out_len
+            (Ghost.reveal input_contents)
+            (Ghost.reveal old_out) **
+          pure (
+            CPI.buffers_wf
+              (Ghost.reveal input_contents)
+              input_len
+              (Ghost.reveal old_out)
+              out_len));
+
+  pe_finish_network_action:
+    i:impl ->
+    cfg:pe_config ->
+    frame:pe_frame ->
+    network_frame:protocol.CPI.pi_network_frame ->
+    result:CPI.process_result ->
+    input_contents:Ghost.erased TCP.bytes ->
+    input_len:SZ.t ->
+    old_out:Ghost.erased TCP.bytes ->
+    out_contents:Ghost.erased TCP.bytes ->
+    st0:Ghost.erased state ->
+    st1:Ghost.erased state ->
+    consumed:Ghost.erased TCP.bytes ->
+    wire_outputs:Ghost.erased (list wire_message) ->
+    local_outputs:Ghost.erased (list local_output) ->
+      stt unit
+        (pe_network_continuation
+          i
+          cfg
+          frame
+          (Ghost.reveal st0)
+          network_frame **
+         protocol.CPI.pi_network_frame_post
+          network_frame
+          result
+          (Ghost.reveal input_contents)
+          input_len
+          (Ghost.reveal old_out)
+          (Ghost.reveal out_contents)
+          (Ghost.reveal st0)
+          (Ghost.reveal st1)
+          (Ghost.reveal consumed)
+          (Ghost.reveal wire_outputs)
+          (Ghost.reveal local_outputs))
+        (fun _ ->
+          pe_frame_ready
+            i
+            cfg
+            frame
+            (Ghost.reveal st1));
+
+  pe_prepare_local_action:
+    i:impl ->
+    cfg:pe_config ->
+    frame:pe_frame ->
+    ev:local_event ->
+    local_frame:protocol.CPI.pi_local_frame ->
+    out:array U8.t ->
+    out_len:SZ.t ->
+    st:Ghost.erased state ->
+    old_out:Ghost.erased TCP.bytes ->
+      stt unit
+        (pe_action_frame
+          i
+          cfg
+          frame
+          (Ghost.reveal st)
+          (EndpointLocal ev local_frame) **
+         local_output_buffer
+          out
+          out_len
+          (Ghost.reveal old_out))
+        (fun _ ->
+          protocol.CPI.pi_local_frame_pre
+            ev
+            local_frame
+            (Ghost.reveal st)
+            out
+            out_len
+            (Ghost.reveal old_out) **
+          pe_local_continuation
+            i
+            cfg
+            frame
+            (Ghost.reveal st)
+            ev
+            local_frame **
+          local_output_buffer
+            out
+            out_len
+            (Ghost.reveal old_out));
+
+  pe_finish_local_action:
+    i:impl ->
+    cfg:pe_config ->
+    frame:pe_frame ->
+    ev:local_event ->
+    local_frame:protocol.CPI.pi_local_frame ->
+    result:CPI.process_result ->
+    old_out:Ghost.erased TCP.bytes ->
+    out_contents:Ghost.erased TCP.bytes ->
+    st0:Ghost.erased state ->
+    st1:Ghost.erased state ->
+    wire_outputs:Ghost.erased (list wire_message) ->
+    local_outputs:Ghost.erased (list local_output) ->
+      stt unit
+        (pe_local_continuation
+          i
+          cfg
+          frame
+          (Ghost.reveal st0)
+          ev
+          local_frame **
+         protocol.CPI.pi_local_frame_post
+          ev
+          local_frame
+          result
+          (Ghost.reveal old_out)
+          (Ghost.reveal out_contents)
+          (Ghost.reveal st0)
+          (Ghost.reveal st1)
+          (Ghost.reveal wire_outputs)
+          (Ghost.reveal local_outputs))
+        (fun _ ->
+          pe_frame_ready
+            i
+            cfg
+            frame
+            (Ghost.reveal st1));
+
+  pe_network_io:
+    Type0;
+
+  pe_network_io_continuation:
+    impl ->
+    pe_channel ->
+    pe_frame ->
+    TCP.bytes ->
+    TCP.bytes ->
+    state ->
+    pe_network_io ->
+    slprop;
+
+  pe_network_input:
+    pe_network_io ->
+    array U8.t;
+
+  pe_network_input_len:
+    pe_network_io ->
+    SZ.t;
+
+  pe_network_output:
+    pe_network_io ->
+    array U8.t;
+
+  pe_network_output_len:
+    pe_network_io ->
+    SZ.t;
+
+  pe_network_input_contents:
+    pe_network_io ->
+    Ghost.erased TCP.bytes;
+
+  pe_network_old_output:
+    pe_network_io ->
+    Ghost.erased TCP.bytes;
+
+  pe_prepare_network_io:
+    i:impl ->
+    ch:pe_channel ->
+    frame:pe_frame ->
+    received:Ghost.erased TCP.bytes ->
+    sent:Ghost.erased TCP.bytes ->
+    st:Ghost.erased state ->
+      stt pe_network_io
+        (pe_io_ready
+          i
+          ch
+          frame
+          (Ghost.reveal received)
+          (Ghost.reveal sent)
+          (Ghost.reveal st))
+        (fun nio ->
+          pe_network_io_continuation
+            i
+            ch
+            frame
+            (Ghost.reveal received)
+            (Ghost.reveal sent)
+            (Ghost.reveal st)
+            nio **
+          network_buffers
+            (pe_network_input nio)
+            (pe_network_input_len nio)
+            (pe_network_output nio)
+            (pe_network_output_len nio)
+            (Ghost.reveal (pe_network_input_contents nio))
+            (Ghost.reveal (pe_network_old_output nio)));
+
+  pe_finish_network_io:
+    i:impl ->
+    ch:pe_channel ->
+    frame:pe_frame ->
+    nio:pe_network_io ->
+    result:CPI.process_result ->
+    received0:Ghost.erased TCP.bytes ->
+    sent0:Ghost.erased TCP.bytes ->
+    st0:Ghost.erased state ->
+    received1:Ghost.erased TCP.bytes ->
+    sent1:Ghost.erased TCP.bytes ->
+    st1:Ghost.erased state ->
+    out_contents:Ghost.erased TCP.bytes ->
+    consumed:Ghost.erased TCP.bytes ->
+    wire_outputs:Ghost.erased (list wire_message) ->
+    local_outputs:Ghost.erased (list local_output) ->
+      stt unit
+        (pe_network_io_continuation
+          i
+          ch
+          frame
+          (Ghost.reveal received0)
+          (Ghost.reveal sent0)
+          (Ghost.reveal st0)
+          nio **
+         pts_to
+          (pe_network_input nio)
+          (Ghost.reveal (pe_network_input_contents nio)) **
+         pts_to
+          (pe_network_output nio)
+          (Ghost.reveal out_contents) **
+         pure (
+          CPI.network_process_correct
+            (protocol.CPI.pi_system i)
+            (Ghost.reveal (pe_network_input_contents nio))
+            (pe_network_input_len nio)
+            (Ghost.reveal (pe_network_old_output nio))
+            (Ghost.reveal out_contents)
+            (pe_network_output_len nio)
+            (Ghost.reveal received0)
+            (Ghost.reveal sent0)
+            (Ghost.reveal st0)
+            result
+            (Ghost.reveal received1)
+            (Ghost.reveal sent1)
+            (Ghost.reveal st1)
+            (Ghost.reveal consumed)
+            (Ghost.reveal wire_outputs)
+            (Ghost.reveal local_outputs)))
+        (fun _ ->
+          pe_io_ready
+            i
+            ch
+            frame
+            (Ghost.reveal received1)
+            (Ghost.reveal sent1)
+            (Ghost.reveal st1));
+
+  pe_local_io:
+    Type0;
+
+  pe_local_io_continuation:
+    impl ->
+    pe_channel ->
+    pe_frame ->
+    TCP.bytes ->
+    TCP.bytes ->
+    state ->
+    local_event ->
+    pe_local_io ->
+    slprop;
+
+  pe_local_output:
+    pe_local_io ->
+    array U8.t;
+
+  pe_local_output_len:
+    pe_local_io ->
+    SZ.t;
+
+  pe_local_old_output:
+    pe_local_io ->
+    Ghost.erased TCP.bytes;
+
+  pe_prepare_local_io:
+    i:impl ->
+    ch:pe_channel ->
+    frame:pe_frame ->
+    ev:local_event ->
+    received:Ghost.erased TCP.bytes ->
+    sent:Ghost.erased TCP.bytes ->
+    st:Ghost.erased state ->
+      stt pe_local_io
+        (pe_io_ready
+          i
+          ch
+          frame
+          (Ghost.reveal received)
+          (Ghost.reveal sent)
+          (Ghost.reveal st))
+        (fun lio ->
+          pe_local_io_continuation
+            i
+            ch
+            frame
+            (Ghost.reveal received)
+            (Ghost.reveal sent)
+            (Ghost.reveal st)
+            ev
+            lio **
+          local_output_buffer
+            (pe_local_output lio)
+            (pe_local_output_len lio)
+            (Ghost.reveal (pe_local_old_output lio)));
+
+  pe_finish_local_io:
+    i:impl ->
+    ch:pe_channel ->
+    frame:pe_frame ->
+    lio:pe_local_io ->
+    ev:local_event ->
+    result:CPI.process_result ->
+    received0:Ghost.erased TCP.bytes ->
+    sent0:Ghost.erased TCP.bytes ->
+    st0:Ghost.erased state ->
+    received1:Ghost.erased TCP.bytes ->
+    sent1:Ghost.erased TCP.bytes ->
+    st1:Ghost.erased state ->
+    out_contents:Ghost.erased TCP.bytes ->
+    wire_outputs:Ghost.erased (list wire_message) ->
+    local_outputs:Ghost.erased (list local_output) ->
+      stt unit
+        (pe_local_io_continuation
+          i
+          ch
+          frame
+          (Ghost.reveal received0)
+          (Ghost.reveal sent0)
+          (Ghost.reveal st0)
+          ev
+          lio **
+         pts_to
+          (pe_local_output lio)
+          (Ghost.reveal out_contents) **
+         pure (
+          CPI.local_process_correct
+            (protocol.CPI.pi_system i)
+            ev
+            (Ghost.reveal (pe_local_old_output lio))
+            (Ghost.reveal out_contents)
+            (pe_local_output_len lio)
+            (Ghost.reveal received0)
+            (Ghost.reveal sent0)
+            (Ghost.reveal st0)
+            result
+            (Ghost.reveal received1)
+            (Ghost.reveal sent1)
+            (Ghost.reveal st1)
+            (Ghost.reveal wire_outputs)
+            (Ghost.reveal local_outputs)))
+        (fun _ ->
+          pe_io_ready
+            i
+            ch
+            frame
+            (Ghost.reveal received1)
+            (Ghost.reveal sent1)
+            (Ghost.reveal st1));
+}
